theories/L/Datatypes/LOptions.v
@@ -5,12 +5,15 @@ Import L_Notations.
 (* ** Encoding of option type *)
 Section Fix_X.
   Variable X:Type.
-  Context {intX : registered X}.
+  Context {intX : encodable X}.
 
 
   MetaCoq Run (tmGenEncode "option_enc" (option X)).
   Hint Resolve option_enc_correct : Lrewrite.
 
+  Global Instance encInj_option_enc {H : encInj intX} : encInj (encodable_option_enc).
+  Proof. register_inj. Qed. 
+  
   (* now we must register the non-constant constructors*)
 
   Global Instance term_Some : computableTime' (@Some X) (fun _ _ => (1,tt)).
@@ -65,7 +68,7 @@ End option_eqb.
 Section int.
 
   Variable X:Type.
-  Context {HX : registered X}.
+  Context {HX : encodable X}.
 
   Global Instance term_option_eqb : computableTime' (@option_eqb X)
                                                     (fun eqb eqbT => (1, fun a _ => (1,fun b _ => (match a,b with
@@ -87,14 +90,11 @@ Section int.
     evar (c:nat). exists c. unfold option_eqb. 
     unfold enc;cbn.
     change (eqb0) with (eqb (X:=X)).
-    extract. unfold eqb,eqbTime. fold (enc (X:=X)).
+    extract. unfold eqb,eqbTime.
     recRel_prettify2. easy.
     [c]:exact (c__eqbComp X + 6).
-    all:unfold c. all:cbn iota beta delta [option_enc].
-    all:  change ((match HX with
-           | @mk_registered _ enc _ _ => enc
-           end)) with (enc (X:=X)).
-    all:cbn [size]. all: nia.
+    all:set (f:=enc (X:=option X)); unfold enc in f;subst f;cbn [size].
+    all:unfold c. all:nia. 
   Qed.
 
 End int.
@@ -102,19 +102,15 @@ End int.
 Definition isSome {T} (u : option T) := match u with Some _ => true | _ => false end.
 
 #[global]
-Instance term_isSome {T} `{registered T} : computable (@isSome T).
+Instance term_isSome {T} `{encodable T} : computable (@isSome T).
 Proof.
   extract.
 Qed.
 
 
-Lemma size_option X `{registered X} (l:option X):
+Lemma size_option X `{encodable X} (l:option X):
   size (enc l) = match l with Some x => size (enc x) + 5 | _ => 3 end.
 Proof.
-  change (enc l) with (option_enc l).
-  destruct l. all:cbn [option_enc map sumn size].
-  change ((match H with
-           | @mk_registered _ enc _ _ => enc
-           end x)) with (enc x).
-  all:lia. 
+  unfold enc at 1.
+  destruct l. all:cbn; nia.
 Qed.
