theories/L/Functions/Equality.v
@@ -34,9 +34,9 @@ Global
 Instance eqbComp_nat : eqbCompT term.
 Proof.
   evar (c:nat). exists c. unfold term_eqb.
-  unfold enc;cbn. unfold term_enc.
-  extract. unfold eqb,eqbTime.
+  extract. unfold eqb,eqbTime. cbn - ["+"].
   [c]:exact (5 + c__eqbComp nat).
-  all:unfold c. set (c__eqbComp nat). change (LNat.nat_enc) with (enc (X:=nat)).
-  solverec. all:try nia. 
+  all:unfold c. set (c__eqbComp nat). 
+  solverec. all: set (f:=enc (X:=term)); unfold enc in f;subst f;cbn [size encodable_term_enc].
+  all:try nia. 
 Qed.
