theories/TM/L/Transcode/BoollistEnc.v
@@ -20,9 +20,9 @@ Definition enc_bool_nil := [lamT; lamT; varT 1; retT; retT].
 Definition enc_bool_closing :=  [appT; retT; retT].
 
 Lemma enc_bool_explicit (bs : list bool):
-  compile (Computable.enc bs) = flat_map enc_bool_perElem bs ++ enc_bool_nil ++ concat (repeat enc_bool_closing (length bs)).
+  compile (enc bs) = flat_map enc_bool_perElem bs ++ enc_bool_nil ++ concat (repeat enc_bool_closing (length bs)).
 Proof.
-  unfold Computable.enc. cbn. unfold Lists.list_enc. cbn. unfold LBool.bool_enc.
+  repeat unfold enc;cbn.
   induction bs as [ | b bs]. reflexivity.
   cbn - [concat repeat]. rewrite IHbs. replace (S (| bs |)) with (|bs|+1) by nia.
   destruct b;cbn - [concat repeat]. all:repeat (autorewrite with list; cbn - [concat repeat]). all:repeat f_equal.
